Rewrite Memory.write_u256()
This method is used by MSTORE, and was suspected of being the reason
for the very poor MSTORE performance.  The method original used
bitvectors to do the necessary shifting.  However, this turns out to a
poor choice and straightforward arithmetic based on division and
remainder is far more efficient (in Z3).

This change now means the sample contract in test.dfy passes
verification, though there are still some unresolved questions.  For
example, why we cannot prove the size of the resulting returndata is
0x20.

src/dafny/util/int.dfy
@@ -57,26 +57,26 @@ module Int {
   // Conversion to/from byte sequences
   // =========================================================
 
-  function read_u8(bytes: seq<u8>, address:nat) : u8
+  function method read_u8(bytes: seq<u8>, address:nat) : u8
   requires address < |bytes| {
     bytes[address]
   }
 
-  function read_u16(bytes: seq<u8>, address:nat) : u16
+  function method read_u16(bytes: seq<u8>, address:nat) : u16
   requires (address+1) < |bytes| {
     var b1 := bytes[address] as u16;
     var b2 := bytes[address+1] as u16;
     (b1 * (TWO_8 as u16)) + b2
   }
 
-  function read_u32(bytes: seq<u8>, address:nat) : u32
+  function method read_u32(bytes: seq<u8>, address:nat) : u32
   requires (address+3) < |bytes| {
     var b1 := read_u16(bytes, address) as u32;
     var b2 := read_u16(bytes, address+2) as u32;
     (b1 * (TWO_16 as u32)) + b2
   }
 
-  function read_u64(bytes: seq<u8>, address:nat) : u64
+  function method read_u64(bytes: seq<u8>, address:nat) : u64
   requires (address+7) < |bytes| {
     var b1 := read_u32(bytes, address) as u64;
     var b2 := read_u32(bytes, address+4) as u64;
