src/dafny/test.dfy
@@ -5,10 +5,10 @@ import opened EVM
 
 // Check most simple program possible
 method test_01(gas: nat) returns (returndata: seq<u8>)
-ensures |returndata| == 0x20
-ensures Int.read_u8(returndata,0) == 0x7b {
+ensures |returndata| > 31
+ensures Int.read_u8(returndata,31) == 0x7b {
   // Initialise EVM
-  var vm := EVM.create(map[],gas,[PUSH1, 0x7b, PUSH1, 0x00, MSTORE8, PUSH1, 0x20, PUSH1, 0x00, RETURN]);
+  var vm := EVM.create(map[],gas,[PUSH1, 0x7b, PUSH1, 0x00, MSTORE, PUSH1, 0x20, PUSH1, 0x00, RETURN]);
   // PUSH1 0x7b
   vm := unwrap(EVM.execute(vm));
   // PUSH1 0x00
