src/dafny/util/memory.dfy
@@ -45,42 +45,6 @@ module Memory {
           0
     }
 
-    function method write_bv16(mem:T, address:u256, val:bv16) : T
-    // Cannot write passed end of memory.
-    requires (address as int) + 1 <= MAX_UINT256 {
-      var lb := (val & 0xFF) as u8;
-      var hb := (val >> 8) as u8;
-      Memory(contents:=mem.contents[address:=hb][address+1:=lb])
-    }
-
-    function method write_bv32(mem:T, address:u256, val:bv32) : T
-    // Cannot write passed end of memory.
-    requires (address as int) + 3 <= MAX_UINT256 {
-      var mem' := write_bv16(mem,address,(val >> 16) as bv16);
-      write_bv16(mem',address+2,(val & 0xFFFF) as bv16)
-    }
-
-    function method write_bv64(mem:T, address:u256, val:bv64) : T
-    // Cannot write passed end of memory.
-    requires (address as int) + 7 <= MAX_UINT256 {
-      var mem' := write_bv32(mem,address,(val >> 32) as bv32);
-      write_bv32(mem',address+4,(val & 0xFFFF_FFFF) as bv32)
-    }
-
-    function method write_bv128(mem:T, address:u256, val:bv128) : T
-    // Cannot write passed end of memory.
-    requires (address as int) + 15 <= MAX_UINT256 {
-      var mem' :=write_bv64(mem,address,(val >> 64) as bv64);
-      write_bv64(mem',address+8,(val & 0xFFFF_FFFF_FFFF_FFFF) as bv64)
-    }
-
-    function method write_bv256(mem:T, address:u256, val:bv256) : T
-    // Cannot write passed end of memory.
-    requires (address as int) + 31 <= MAX_UINT256 {
-      var mem' := write_bv128(mem,address,(val >> 128) as bv128);
-      write_bv128(mem',address+16,(val & 0xFFFF_FFFF_FFFF_FFFF_FFFF_FFFF_FFFF_FFFF) as bv128)
-    }
-
     /**
      * Write a byte to a given address in Memory.
      */
@@ -89,10 +53,64 @@ module Memory {
         Memory(contents:=mem.contents[address:=val])
     }
 
+    /**
+     * Write a 16bit word to a given address in Memory using
+     * big-endian addressing.
+     */
+    function method write_u16(mem:T, address:u256, val:u16) : T
+    requires (address as int) + 1 <= MAX_UINT256 {
+      var b1 := val / (TWO_8 as u16);
+      var b2 := val % (TWO_8 as u16);
+      var mem' := write_u8(mem,address,b1 as u8);
+      write_u8(mem,address+1,b2 as u8)
+    }
+
+    /**
+     * Write a 32bit word to a given address in Memory using
+     * big-endian addressing.
+     */
+    function method write_u32(mem:T, address:u256, val:u32) : T
+    requires (address as int) + 3 <= MAX_UINT256 {
+      var b1 := val / (TWO_16 as u32);
+      var b2 := val % (TWO_16 as u32);
+      var mem' := write_u16(mem,address,b1 as u16);
+      write_u16(mem,address+2,b2 as u16)
+    }
+
+    /**
+     * Write a 64bit word to a given address in Memory using
+     * big-endian addressing.
+     */
+    function method write_u64(mem:T, address:u256, val:u64) : T
+    requires (address as int) + 7 <= MAX_UINT256 {
+      var b1 := val / (TWO_32 as u64);
+      var b2 := val % (TWO_32 as u64);
+      var mem' := write_u32(mem,address,b1 as u32);
+      write_u32(mem,address+4,b2 as u32)
+    }
+
+    /**
+     * Write a 128bit word to a given address in Memory using
+     * big-endian addressing.
+     */
+    function method write_u128(mem:T, address:u256, val:u128) : T
+    requires (address as int) + 15 <= MAX_UINT256 {
+      var b1 := val / (TWO_64 as u128);
+      var b2 := val % (TWO_64 as u128);
+      var mem' := write_u64(mem,address,b1 as u64);
+      write_u64(mem,address+8,b2 as u64)
+    }
+
+    /**
+     * Write a 256bit word to a given address in Memory using
+     * big-endian addressing.
+     */
     function method write_u256(mem:T, address:u256, val:u256) : T
-    // Cannot write passed end of memory.
     requires (address as int) + 31 <= MAX_UINT256 {
-      write_bv256(mem,address,val as bv256)
+      var b1 := val / (TWO_128 as u256);
+      var b2 := val % (TWO_128 as u256);
+      var mem' := write_u128(mem,address,b1 as u128);
+      write_u128(mem,address+16,b2 as u128)
     }
 
     /**
